Assignment_06.thy
@@ -2,12 +2,182 @@ theory Assignment_06
   imports Main
 begin
 
-datatype aexp = Const | Var string |Plus aexp aexp
 
-fun aval :: "aexp => state => val" where
+(* exercise 3.3 *)
+type_synonym vname = string
+datatype aexp = N int | V vname | Plus aexp aexp
+
+type_synonym val = int
+type_synonym state = "vname \<Rightarrow> val" 
 
 
 definition null_state ("<>") where
   "null_state \<equiv>  \<lambda>x. 0"
+
+
+fun aval :: "aexp \<Rightarrow> state \<Rightarrow> val" where
+  "aval (N n) s = n" 
+| "aval (V x ) s = s x" 
+| "aval (Plus a1 a2) s = aval a1 s + aval a2 s"
+
+value "aval (Plus (N 3) (V '' x '')) (\<lambda>x . 0)"
+
+
+fun asimp_const :: "aexp \<Rightarrow> aexp" where
+  "asimp_const (N n) = N n" 
+| "asimp_const (V x) = V x"
+| "asimp_const  (Plus a1 a2) = (case (asimp_const a1, asimp_const a2) of (N n1, N n2) \<Rightarrow> N(n1 + n2)
+  | (b1, b2) \<Rightarrow> Plus b1 b2)"
+
+(*subst x a e is the result of replacing every
+occurrence of variable x by a in e*)
+fun subst :: "vname \<Rightarrow> aexp \<Rightarrow> aexp \<Rightarrow> aexp" where
+  "subst x a1 (N n) = N n"
+| "subst x a1 (V y)  = (if x = y then a1 else V y)"
+| "subst x a1 (Plus e1 e2) = Plus (subst x a1 e1) (subst x a1 e2)"
+
+value "subst ''x'' (N 3) (Plus (V ''x'')(V ''y''))"
+
+lemma "aval (subst x a e) s = aval e (s(x := aval a s))"
+  apply (induction e arbitrary: x)
+    apply (auto)
+  done
+
+(*exercise 3.4*)
+datatype aexp1 = N int | V vname | Plus aexp1 aexp1 | Times aexp1 aexp1
+
+fun aval1 :: "aexp1 \<Rightarrow> state \<Rightarrow> val" where
+  "aval1 (N n) s = n" 
+| "aval1 (V x ) s = s x" 
+| "aval1 (Plus a1 a2) s = aval1 a1 s + aval1 a2 s"
+| "aval1 (Times a1 a2) s = aval1 a1 s * aval1 a2 s"
+
+fun plus1 :: "aexp1 \<Rightarrow> aexp1 \<Rightarrow> aexp1" where
+  "plus1 (N i1) (N i2) = N (i1 + i2)"
+| "plus1 (N i) a  = (if i=0 then a else Plus (N i) a)"
+| "plus1 a (N i) = (if i=0 then a else Plus a (N i))"
+| "plus1 a1 a2 = Plus a1 a2"
+
+fun times :: "aexp1 \<Rightarrow> aexp1 \<Rightarrow> aexp1" where
+  "times (N i1) (N i2) = N (i1 * i2)"
+| "times (N i) a  = (if i=0 then N 0 else (if i=1 then a else Times (N i) a))"
+| "times a (N i) = (if i=0 then N 0 else (if i=1 then a else Times a (N i)))"
+| "times a1 a2 = Times a1 a2"
+
+fun asimp1 :: "aexp1 \<Rightarrow> aexp1" where
+  "asimp1 (N n) = N n"
+| "asimp1 (V x) = V x"
+| "asimp1 (Plus a1 a2) = plus1 (asimp1 a1) (asimp1 a2)"
+| "asimp1 (Times a1 a2) = times (asimp1 a1) (asimp1 a2)"
+
+lemma aval_plus1  [simp]: "aval1 (plus1 a1 a2) s = aval1 a1 s + aval1 a2 s"
+  apply(induction a1 rule: plus1.induct)
+    apply (auto)
+  done
+
+lemma aval_times  [simp]: "aval1 (times a1 a2) s = aval1 a1 s * aval1 a2 s"
+  apply(induction a1 rule: times.induct)
+    apply (auto)
+  done
+
+lemma "aval1 (asimp1 a) s = aval1 a s"
+  apply (induction a)
+     apply (auto)
+  done
+
+(*exercise 3.7*)
+
+(* boolean constants, negation, conjunction and comparison of expressions for less-than*)
+datatype bexp= Bc bool | Not bexp | And bexp bexp | Less aexp aexp
+
+
+fun bval :: "bexp \<Rightarrow> state \<Rightarrow> bool" where
+  "bval (Bc v) s = v"
+| "bval (Not b) s = (\<not> bval b s)"
+| "bval (And b1 b2) s = (bval b1 s \<and> bval b2 s)"
+| "bval (Less a1 a2) s = (aval a1 s < aval a2 s)"
+
+
+fun not :: "bexp \<Rightarrow> bexp" where
+  "not (Bc True) = Bc False"
+| "not (Bc False) = Bc True"
+| "not b = Not b"
+
+fun "and" :: "bexp \<Rightarrow> bexp \<Rightarrow> bexp" where
+  "and (Bc True) b = b"
+| "and b (Bc True) = b"
+| "and (Bc False) b = Bc False"
+| "and b (Bc False) = Bc False"
+| "and b1 b2 = And b1 b2"
+
+fun less :: "aexp \<Rightarrow> aexp \<Rightarrow> bexp" where
+  "less (N n1) (N n2) = Bc(n1 < n2)"
+| "less a1 a2  = Less a1 a2"
+
+fun bsimp :: "bexp \<Rightarrow> bexp" where
+  "bsimp (Bc v) = Bc v"
+| "bsimp (Not b) = not(bsimp b)" 
+| "bsimp (And b1 b2) = and (bsimp b1) (bsimp b2)" 
+| "bsimp (Less a1 a2) = less (asimp a1) (asimp a2)"
+
+defintion Le :: "aexp \<Rightarrow> aexp \<Rightarrow> bexp" where
+  ""
+
+(*exercise 3.9*)
+
+datatype pbexp =
+VAR vname | NEG pbexp | AND pbexp pbexp | OR pbexp pbexp
+
+fun pbval :: "pbexp \<Rightarrow> (vname \<Rightarrow> bool) \<Rightarrow> bool" where
+  "pbval (VAR x ) s = s x"
+| "pbval (NEG b) s = (\<not> pbval b s)" 
+| "pbval (AND b1 b2) s = (pbval b1 s \<and> pbval b2 s)" 
+| "pbval (OR b1 b2) s = (pbval b1 s \<or> pbval b2 s)"
+
+
+fun is_nnf :: "pbexp \<Rightarrow> bool" where
+  "is_nnf (VAR x) = True"
+| "is_nnf (NEG (VAR x)) = True"
+| "is_nnf (NEG _) = False"
+| "is_nnf (AND b1 b2) = ((is_nnf b1)\<and> (is_nnf b2))"
+| "is_nnf (OR b1 b2) = ((is_nnf b1) \<and> (is_nnf b2))"
+
+
+fun nnf :: "pbexp \<Rightarrow> pbexp" where
+  "nnf (VAR x) = VAR x"
+| "nnf (NEG (VAR x)) = (NEG (VAR x))"
+| "nnf (NEG (NEG (b1))) = nnf b1"
+| "nnf (AND b1 b2) = AND (nnf b1) (nnf b2)"
+| "nnf (OR b1 b2) = OR (nnf b1) (nnf b2)"
+| "nnf (NEG (AND b1 b2)) = OR (nnf (NEG b1)) (nnf (NEG b2))"
+| "nnf (NEG (OR b1 b2)) = AND (nnf (NEG b1)) (nnf (NEG b2))"
+
+
+
+lemma "pbval (nnf b) s = pbval b s"
+  apply (induction b rule: nnf.induct )
+        apply (auto)
+  done
+
+lemma "(is_nnf (nnf b))"
+  apply (induction b rule: nnf.induct)
+        apply (auto)
+  done
+
+fun OR_check :: "pbexp \<Rightarrow> bool" where
+  "OR_check (OR b1 b2) = False"
+| "OR_check (AND b1 b2) = ((OR_check b1) \<and> (OR_check b2))"
+| "OR_check _ = True "
+
+fun is_dnf :: "pbexp \<Rightarrow> bool" where
+  "is_dnf (AND b1 b2) = (((is_nnf b1) \<and> (OR_check b1)) \<and> ((is_nnf b2) \<and> (OR_check b2)))"
+| "is_dnf (OR b1 b2) = ((is_dnf b1) \<and> (is_dnf b2))"
+| "is_dnf b1  = is_nnf b1"
+
+fun dnf_of_nnf :: "" where
+
+(* exercise 3.11*)
+
+
 
 end
