Exercise_7_1.thy
@@ -1,0 +1,5 @@
+theory Exercise_7_1
+  imports Big_Step
+begin
+
+end
