Options.thy
@@ -1,0 +1,62 @@
+theory Options
+  imports Main
+begin
+
+type_synonym vname = string
+datatype aexp = N int | V vname | Plus aexp aexp
+
+type_synonym val = int
+type_synonym state = "vname \<Rightarrow> val" 
+
+
+datatype instr = LOADI val | LOAD vname | ADD
+
+type_synonym stack = "val list"
+
+fun exec1 :: "instr \<Rightarrow> state \<Rightarrow> stack \<Rightarrow> stack" where
+"exec1 (LOADI n) _ stk = n # stk" |
+"exec1 (LOAD x ) s stk = s(x ) # stk" |
+"exec1 ADD _ (j # i # stk) = (i + j) # stk"
+
+fun exec :: "instr list \<Rightarrow> state \<Rightarrow> stack \<Rightarrow> stack" where
+"exec [] _ stk = stk" |
+"exec (i#is) s stk = exec is s (exec1 i s stk)"
+
+fun comp :: "aexp \<Rightarrow> instr list" where
+"comp (N n) = [LOADI n]" |
+"comp (V x ) = [LOAD x ]" |
+"comp (Plus e1 e2) = comp e1 @ comp e2 @ [ADD]"
+
+
+lemma "exec (comp a) s stk = aval a s # stk "
+  apply (induction a)
+
+lemma exec_append: ""
+
+(*exercise 3.10*)
+
+(*need to define hd2 and tl2*)
+fun exec1' :: "instr \<Rightarrow> state \<Rightarrow> stack \<Rightarrow> stack option" where
+  "exec1' (LOADI n) _ stk = Some (n # stk)"
+| "exec1' (LOADI x) s stk = Some ((s x) # stk)"
+| "exec1' ADD _ [] = None"
+| "exec1' ADD _ [_] = None"
+| "exec1' ADD _ stk = Some ((hd2 stk + hd stk) # tl2 stk)"
+
+
+fun exec' :: "instr list \<Rightarrow> state \<Rightarrow> stack \<Rightarrow> stack" where
+"exec' [] _ stk = Some stk" |
+"exec' (i#is) s stk = (case (exec1 i s stk) of
+                        None \<Rightarrow> None
+                      | Some new_stk \<Rightarrow> exec' is s new_stk)"
+
+lemma exec'_append: "exec' is1 s stk = Some new_stk \<Longrightarrow> exec' (is1 @ is2) s stk = exec' is2 s new_stk"
+  apply (induction is1 arbitrary: stk)
+  apply(auto split: option.split)
+  done
+
+lemma "exec' (comp a) s stk = Some (aval a s # stk)"
+  apply (induction a arbitrary: stk)
+  by (auto simp add: exec'_append)
+
+end
